wip

src/Arithmetic/P256ADX.v
@@ -7,13 +7,18 @@ Require Import Crypto.Arithmetic.WeightStream.
 Import WeightStream.Saturated.
 Import Crypto.Util.ZUtil.Definitions.
 Import Crypto.Util.LetIn.
+Require Import Crypto.Util.Bool.
 
 Definition p256 := 0xffffffff00000001000000000000000000000000ffffffffffffffffffffffff%Z.
 Definition p3 :=   0xffffffff00000001%Z.
 
 Definition n : nat := 4.
-Definition bound (_ : nat) : positive := Z.to_pos (2^64).
+Definition bound : positive := Z.to_pos (2^64).
 Local Notation eval := (eval bound).
+
+Lemma if_expect_true_to_if_negb {A} b (t:A) (f:unit->A) :
+  if_expect_true b t f = if negb b then f tt else t.
+Proof. destruct b; reflexivity. Time Qed.
 
 Definition two_steps_of_p256_montgomery_reduction xs :=
   let x := hd 0 xs in
@@ -46,54 +51,82 @@ Definition p256_sqr' a :=
   dlet a := two_steps_of_p256_montgomery_reduction a in
   dlet a := two_steps_of_p256_montgomery_reduction a in
   dlet a := condsub bound a (encode bound 4 p256) in
-  dlet a := firstn 4 a in
-  a.
+  firstn 4 a.
 
 (* Versions with bounds-checking assertions *)
 
 Definition p256_mul x y :=
-  if negb (2 <=? Z.of_nat (Datatypes.length x)) then nil else
-  if negb ((0 <=? eval x) && (eval x <? 2^256)) then nil else
-  if negb ((0 <=? eval y) && (eval y <? 2^256)) then nil else
-  dlet xlo := firstn 2 x in
-  dlet xhi := skipn 2 x in
-  if negb ((0 <=? eval xlo) && (eval xlo <? 2^128)) then nil else
-  dlet a := mul bound (firstn 2 x) y in
-  if negb ((0 <=? hd 0 a) && (hd 0 a <? 2 ^ 64)) then nil else
-  if negb ((0 <=? hd 0 (tl a)) && (hd 0 (tl a) <? 2 ^ 64)) then nil else
-  dlet a := two_steps_of_p256_montgomery_reduction a in
-  if negb ((0 <=? eval xhi) && (eval xhi <? 2^128)) then nil else
-  dlet a := add_mul bound a xhi y in
-  if negb ((0 <=? hd 0 a) && (hd 0 a <? 2 ^ 64)) then nil else
-  if negb ((0 <=? hd 0 (tl a)) && (hd 0 (tl a) <? 2 ^ 64)) then nil else
-  dlet a := two_steps_of_p256_montgomery_reduction a in
-  if negb (eval a <? (weight bound (Nat.max (Datatypes.length a) (Datatypes.length (encode bound 4 p256))))) then nil else
-  dlet a := condsub bound a (encode bound 4 p256) in
-  if negb (4 <=? Z.of_nat (Datatypes.length a)) then nil else
-  if negb (isbounded bound a) then nil else
-  firstn 4 a.
+  if_expect_true (2 <=? Z.of_nat (Datatypes.length x))
+  (if_expect_true ((0 <=? eval x) && (eval x <? 2^256))
+   (if_expect_true ((0 <=? eval y) && (eval y <? 2^256))
+    (dlet xlo := firstn 2 x in
+     dlet xhi := skipn 2 x in
+     if_expect_true ((0 <=? eval xlo) && (eval xlo <? 2^128))
+     (dlet a := mul bound (firstn 2 x) y in
+      if_expect_true ((0 <=? hd 0 a) && (hd 0 a <? 2 ^ 64))
+      (if_expect_true ((0 <=? hd 0 (tl a)) && (hd 0 (tl a) <? 2 ^ 64))
+       (dlet a := two_steps_of_p256_montgomery_reduction a in
+        if_expect_true ((0 <=? eval xhi) && (eval xhi <? 2^128))
+        (dlet a := add_mul bound a xhi y in
+         if_expect_true ((0 <=? hd 0 a) && (hd 0 a <? 2 ^ 64))
+         (if_expect_true ((0 <=? hd 0 (tl a)) && (hd 0 (tl a) <? 2 ^ 64))
+          (dlet a := two_steps_of_p256_montgomery_reduction a in
+           if_expect_true (eval a <? (weight bound (Nat.max (Datatypes.length a) (Datatypes.length (encode bound 4 p256)))))
+           (dlet a := condsub bound a (encode bound 4 p256) in
+            if_expect_true (4 <=? Z.of_nat (Datatypes.length a))
+            (if_expect_true (isbounded bound a)
+             (firstn 4 a)
+             (fun _ => nil))
+            (fun _ => nil))
+           (fun _ => nil))
+          (fun _ => nil))
+         (fun _ => nil))
+        (fun _ => nil))
+       (fun _ => nil))
+      (fun _ => nil))
+     (fun _ => nil))
+    (fun _ => nil))
+   (fun _ => nil))
+  (fun _ => nil).
 
 Lemma p256_mul'_correct x y : p256_mul x y <> nil -> p256_mul' x y = p256_mul x y.
-Proof. cbv [p256_mul p256_mul' Let_In]; break_match; congruence. Qed.
+Proof.
+  cbv [p256_mul p256_mul' Let_In].
+  rewrite !if_expect_true_to_if_negb.
+  cbn [negb].
+  break_match; congruence.
+Time Qed.
 
 Definition p256_sqr a :=
-  if negb (4 =? Z.of_nat (Datatypes.length a)) then nil else
-  dlet a := sqr4 a in
-  if negb ((0 <=? hd 0 a) && (hd 0 a <? 2 ^ 64)) then nil else
-  if negb ((0 <=? hd 0 (tl a)) && (hd 0 (tl a) <? 2 ^ 64)) then nil else
-  dlet a := two_steps_of_p256_montgomery_reduction a in
-  if negb ((0 <=? hd 0 a) && (hd 0 a <? 2 ^ 64)) then nil else
-  if negb ((0 <=? hd 0 (tl a)) && (hd 0 (tl a) <? 2 ^ 64)) then nil else
-  dlet a := two_steps_of_p256_montgomery_reduction a in
-  if negb (eval a <? (weight bound (Nat.max (Datatypes.length a) (Datatypes.length (encode bound 4 p256))))) then nil else
-  dlet a := condsub bound a (encode bound 4 p256) in
-  if negb (4 <=? Z.of_nat (Datatypes.length a)) then nil else
-  if negb (isbounded bound a) then nil else
-  dlet a := firstn 4 a in
-  a.
+  if_expect_true (4 =? Z.of_nat (Datatypes.length a))
+  (dlet a := sqr4 a in
+   if_expect_true ((0 <=? hd 0 a) && (hd 0 a <? 2 ^ 64))
+   (if_expect_true ((0 <=? hd 0 (tl a)) && (hd 0 (tl a) <? 2 ^ 64))
+    (dlet a := two_steps_of_p256_montgomery_reduction a in
+     if_expect_true ((0 <=? hd 0 a) && (hd 0 a <? 2 ^ 64))
+     (if_expect_true ((0 <=? hd 0 (tl a)) && (hd 0 (tl a) <? 2 ^ 64))
+      (dlet a := two_steps_of_p256_montgomery_reduction a in
+       if_expect_true (eval a <? (weight bound (Nat.max (Datatypes.length a) (Datatypes.length (encode bound 4 p256)))))
+       (dlet a := condsub bound a (encode bound 4 p256) in
+        if_expect_true (4 <=? Z.of_nat (Datatypes.length a))
+        (if_expect_true (isbounded bound a)
+         (firstn 4 a)
+         (fun _ => nil))
+        (fun _ => nil))
+       (fun _ => nil))
+      (fun _ => nil))
+     (fun _ => nil))
+    (fun _ => nil))
+   (fun _ => nil))
+  (fun _ => nil).
 
 Lemma p256_sqr'_correct x : p256_sqr x <> nil -> p256_sqr' x = p256_sqr x.
-Proof. cbv [p256_sqr p256_sqr' Let_In]; break_match; congruence. Qed.
+Proof.
+  cbv [p256_sqr p256_sqr' Let_In].
+  rewrite !if_expect_true_to_if_negb.
+  cbn [negb].
+  break_match; congruence.
+Time Qed.
 
 Lemma two_steps_of_p256_montgomery_reduction_correct xs :
   let z := eval (two_steps_of_p256_montgomery_reduction xs) in
@@ -103,34 +136,40 @@ Lemma two_steps_of_p256_montgomery_reduction_correct xs :
     (eval xs <= (2^256+2^129-2^96)*(2^128-1) -> 0 <= z < 2^256 + p256) /\
     (eval xs <= (2^256-2^223)*(2^256-2^223) -> 0 <= z < 2^128 * p256)).
 Proof.
-  cbv [Let_In two_steps_of_p256_montgomery_reduction].
+  unfold two_steps_of_p256_montgomery_reduction, Let_In.
   pose proof eval_hd_tl bound xs; pose proof eval_hd_tl bound (tl xs).
   set (hd 0 xs) as x in *; set (hd 0 (tl xs)) as y in *.
   rewrite ?eval_cons in *.
-  repeat change (stream.tl ?b) with b in *.
-  repeat change (stream.hd _) with (2^64)%positive in *.
-  edestruct Z.mul_split as (tl, th) eqn:Et.
-  rewrite Z.mul_split_correct in Et; symmetry in Et; Prod.inversion_pair.
-  edestruct Z.add_with_get_carry_full as (x', c) eqn:Ex'.
-  rewrite Z.add_with_get_carry_full_correct in Ex'; symmetry in Ex'; Prod.inversion_pair; rewrite ?Z.add_0_l in *.
+  change (Z.pos bound) with (2^64)%Z in *.
+  rewrite <- H0 in H. clear H0.
+  rewrite Z.mul_split_correct.
+  rewrite Z.add_with_get_carry_full_correct.
+  rewrite ?Z.add_0_l.
+  cbn [fst snd].
   rewrite eval_product_scan_.
   set (_ + _) as z.
-  assert (2 ^ 128 * z = eval xs + (x + 2 ^ 64 * x') * p256) as Hz; [|clearbody z].
-  { subst z.
-    enough (eval (map _ _) = 2^32 * x' + 2^64 * p3 * x + 2^128 * p3*x') as ->.
-    { cbv [p256 p3]; Z.div_mod_to_equations; nia. }
+  assert (2 ^ 128 * z = eval xs + (x + 2 ^ 64 * ((y + (2 ^ 32 * x) mod 2 ^ 64) mod 2 ^ 64)) * p256) as Hz.
+  { unfold z.
+    enough (eval (map (uncurry Z.mul) ([(2 ^ 32, (y + (2 ^ 32 * x) mod 2 ^ 64) mod 2 ^ 64); (p3, x); (p3, (y + (2 ^ 32 * x) mod 2 ^ 64) mod 2 ^ 64)] ++ repeat (0, 0) (length xs - 5))) = 2^32 * ((y + (2 ^ 32 * x) mod 2 ^ 64) mod 2 ^ 64) + 2^64 * p3 * x + 2^128 * p3 * ((y + (2 ^ 32 * x) mod 2 ^ 64) mod 2 ^ 64)) as ->.
+    { cbv [p256 p3] in *; unfold z in *.
+      change (2^64) with 18446744073709551616 in *.
+      change (2^128) with 340282366920938463463374607431768211456 in *.
+      change (2^32) with 4294967296 in *.
+      Z.div_mod_to_equations; lia. }
     rewrite map_app, map_repeat, eval_app, eval_repeat_0.
-    cbn [List.length List.map uncurry eval PreExtra.list_rect_fbb_b list_rect].
-    change (stream.hd _) with (2^64)%positive.
+    cbv [List.length List.map uncurry eval bound ListUtil.list_rect_arrow_nodep ListUtil.list_rect_nodep list_rect fst snd]; change (Z.pos bound) with (2^64)%Z.
     Z.div_mod_to_equations; nia. }
+  clearbody z.
+  set ((y + (2 ^ 32 * x) mod 2 ^ 64) mod 2 ^ 64) as x' in *.
   split; intros.
-  { symmetry; erewrite <-Z.mod_add with (b := x + 2^64*x') by (cbv; lia); symmetry; f_equal; lia. }
-  assert (0 <= 2^128 * z) by (rewrite Hz; cbv [p256]; Z.div_mod_to_equations; lia).
-  assert (0 <= 2^384 -2^352 +2^320 + (x + 2^64 * x')*p256 < 2^128*(p256+p256)) by (cbv [p256]; Z.div_mod_to_equations; lia).
-  assert (0 <= (2^256+2^129-2^96)*(2^128-1) + (x + 2^64 * x')*p256 < 2^128*(p256+2^256)) by (cbv [p256]; Z.div_mod_to_equations; lia).
-  assert (0 <= (2^256-2^223)*(2^256-2^223) + (x + 2^64 * x')*p256 < 2^128*2^128*p256) by (cbv [p256]; Z.div_mod_to_equations; lia).
-  lia.
-Qed.
+  { symmetry; erewrite <-Z.mod_add with (b := x + 2^64*x') by (cbv [p256]; nia); symmetry; f_equal; nia. }
+  assert (0 <= x' < 2^64) by (unfold x'; Z.div_mod_to_equations; nia).
+  assert (0 <= 2^128 * z) by (rewrite Hz; cbv [p256]; nia).
+  assert (0 <= 2^384 -2^352 +2^320 + (x + 2^64 * x')*p256 < 2^128*(p256+p256)) by (cbv [p256]; nia).
+  assert (0 <= (2^256+2^129-2^96)*(2^128-1) + (x + 2^64 * x')*p256 < 2^128*(p256+2^256)) by (cbv [p256]; nia).
+  assert (0 <= (2^256-2^223)*(2^256-2^223) + (x + 2^64 * x')*p256 < 2^128*2^128*p256) by (cbv [p256]; nia).
+  cbv [p256] in *; nia.
+Time Qed.
 
 Ltac lift_let :=
   match goal with
@@ -169,20 +208,22 @@ Proof.
   subst y0 y.
   rewrite eval_product_scan_, eval_product_scan_, ?eval_nil, ?Z.add_0_l.
   cbn [map uncurry]; rewrite ?Z.mul_0_l, ?Z.add_0_r.
-  rewrite ?eval_cons, ?eval_nil in *;
-  progress repeat change (stream.tl ?b) with b in *;
-  progress repeat change (Z.pos (stream.hd bound)) with (2^64) in *;
-  progress repeat change (stream.hd ?b) with (b O) in *; cbv beta in *.
-  change (Z.pos (weight bound 8)) with (2^512) in *.
-  rewrite Z.mod_small; nia.
-Qed.
+  rewrite ?eval_cons, ?eval_nil in *.
+  cbv [eval Saturated.eval bound weight ListUtil.list_rect_arrow_nodep ListUtil.list_rect_nodep list_rect fst snd fold_right repeat] in *.
+  rewrite ?Pos2Z.inj_mul in *.
+  change (Z.pos bound) with (2^64)%Z in *.
+  change (Z.pos (Z.to_pos (2^64))) with (2^64)%Z in *.
+  Z.div_mod_to_equations; nia.
+Time Qed.
+
 
 Lemma eval_p256_mul x y (z := p256_mul x y) (Hcompiles : z <> nil) :
+  length x = 4%nat -> length y = 4%nat ->
   0 <= eval y < p256 ->
   2^256 * eval z mod p256 = eval x * eval y mod p256 /\
   (0 <= eval x < p256 -> 0 <= eval z < p256).
 Proof.
-  intros Hy.
+  intros Hlenx Hleny Hy.
   pose proof firstn_skipn 2 x as H; eapply (f_equal eval) in H.
 
   cbv beta delta [p256_mul Let_In] in *.
@@ -192,6 +233,19 @@ Proof.
   subst y0. subst y1.
   repeat lift_let.
 
+  (*
+  assert (Hlen_y3 : length y3 = 6%nat).
+  { cbv [y3 y2 y1 y0].
+    rewrite length_two_steps_7; [trivial|].
+    rewrite length_add_mul_4_2; [trivial| | |trivial].
+    { rewrite length_two_steps_6; [trivial|].
+      cbv [mul].
+      rewrite length_add_mul_0_2; [trivial| |trivial].
+      { cbv [xlo]. rewrite firstn_length. rewrite Hlenx. cbv. reflexivity. } }
+    { cbv [xlo]. rewrite firstn_length. rewrite Hlenx. cbv. reflexivity. }
+    { cbv [xhi]. rewrite length_skipn. rewrite Hlenx. cbv. reflexivity. }
+  }
+
   repeat match goal with
          | x := ?v |- _ =>
              let H := fresh "H" x in
@@ -199,10 +253,10 @@ Proof.
              move H before x;
              clearbody x
          end.
+  rewrite !if_expect_true_to_if_negb in *.
 
   eapply (f_equal eval) in Hy0.
-  rewrite (eval_mul (Z.to_pos (2^64))) in Hy0.
-  change (fun _ => _) with bound in *.
+  rewrite (eval_mul bound) in Hy0.
   
   repeat match goal with
   | H : context G [match ?x with _ => _ end] |- _ =>
@@ -211,10 +265,9 @@ Proof.
   rewrite Bool.negb_false_iff, Bool.andb_true_iff, Z.leb_le, Z.ltb_lt in *.
 
   rewrite eval_app in H.
-  rewrite 2Hxlo in H at 2.
+  rewrite Hxlo in H at 2.
   rewrite !firstn_length_le in H by lia.
   progress change (Z.pos (weight bound 2)) with (2^128) in *.
-  progress change (stream.skipn _ bound) with bound in *.
 
   pose proof two_steps_of_p256_montgomery_reduction_correct y0 as HH.
   rewrite <-Hy1, Hy0 in HH; clear Hy1; cbv zeta in HH; case HH as [Hy1 HH'1].
@@ -224,24 +277,17 @@ Proof.
   do 1 specialize (HH'1 ltac:(cbv [p256] in *; nia)).
 
   eapply (f_equal eval) in Hy2.
-  rewrite (eval_add_mul (Z.to_pos (2^64))) in Hy2.
-  change (fun _ => _) with bound in *.
+  rewrite (eval_add_mul bound) in Hy2.
 
   pose proof two_steps_of_p256_montgomery_reduction_correct y2 as HH.
   pose proof Hy3 as Hy3'.
   rewrite <-Hy3, Hy2 in HH; clear Hy3; cbv zeta in HH; case HH as [Hy3 HH'2].
 
-  assert (HH : (2 ^ 256 * eval y3) mod p256 =
-    ((2^128 * eval y1) mod p256 + 2^128 * eval xhi * eval y) mod p256).
-  { clear -Hy3; cbv [p256] in *; Z.div_mod_to_equations; nia. }
-  rewrite Hy1 in HH; clear Hy1 Hy3; autorewrite with pull_Zmod in HH.
-  replace (eval xlo * eval y + 2 ^ 128 * eval xhi * eval y)
-    with (eval x * eval y) in HH by nia.
-
   eapply (f_equal eval) in Hy4.
   rewrite eval_condsub, eval_encode, Z.mod_small in Hy4.
   2: { cbv. intuition congruence. }
-  2: { trivial. }
+  2: { rewrite Hlen_y3. rewrite length_encode. cbv; lia. }
+  2: { rewrite Hlen_y3. cbv; lia. }
   2: { cbv. inversion 1. }
   destruct (isbounded_correct bound y4) in *; [|discriminate].
 
@@ -251,7 +297,8 @@ Proof.
   rewrite <-e, eval_firstn_encode in Hz by lia.
   progress change (Z.pos (weight bound 4)) with (2^256) in *.
   rewrite Z.mod_small in Hz; cycle 1.
-  { apply proj2, proj1 in HH'2.
+  { rewrite Hy4.
+    apply proj2, proj1 in HH'2.
     do 1 specialize (HH'2 ltac:(cbv [p256] in *; nia)).
     destruct (Z.leb_spec p256 (eval y3)) in *; simpl Z.b2z in *; cbv [p256] in *; lia. }
 
@@ -259,9 +306,10 @@ Proof.
   split.
   { Modulo.push_Zmod; Modulo.pull_Zmod. rewrite Z.mul_0_r, Z.sub_0_r; trivial. }
   { intros. destruct (Z.leb_spec p256 (eval y3)) in *; simpl Z.b2z in *; cbv [p256] in *; nia. }
-Qed.
+*)
+Time Admitted.
 
-Lemma p256_sqr_sufficient_bound : p256 < 2^256-2^223. Proof. compute. trivial. Qed.
+Lemma p256_sqr_sufficient_bound : p256 < 2^256-2^223. Proof. compute. trivial. Time Qed.
 
 Lemma eval_p256_sqr x (z := p256_sqr x) (Hcompiles : z <> nil) :
   0 <= eval x < 2^256-2^223 ->
@@ -275,11 +323,12 @@ Proof.
   repeat match reverse goal with
          | x := ?v |- _ =>
              let H := fresh "H" x in
-             (* assert (x = v) as H by exact eq_refl; (*COQBUG?: Qed hangs*) *)
+             (* assert (x = v) as H by exact eq_refl; (*COQBUG?: Time Qed.hangs*) *)
              assert (x = v) as H by reflexivity;
              move H before x;
              clearbody x
          end.
+  rewrite !if_expect_true_to_if_negb in *.
   
   repeat match goal with
   | H : context G [match ?x with _ => _ end] |- _ =>
@@ -293,21 +342,22 @@ Proof.
 
   pose proof two_steps_of_p256_montgomery_reduction_correct y as HH.
   rewrite <-Hy1, Hy0 in HH; clear Hy1; cbv zeta in HH; case HH as [Hy1 HH'1].
-  do 3 specialize (HH'1 ltac:(cbv [p256] in *; nia)).
+  do 3 specialize (HH'1 ltac:(cbv [p256 bound] in *; nia)).
   apply proj2, proj2 in HH'1.
-  do 1 specialize (HH'1 ltac:(cbv [p256] in *; nia)).
+  do 1 specialize (HH'1 ltac:(cbv [p256 bound] in *; nia)).
 
   pose proof two_steps_of_p256_montgomery_reduction_correct y0 as HH.
   pose proof Hy2 as Hy2'.
   rewrite <-Hy2 in HH; clear Hy2; cbv zeta in HH; case HH as [Hy2 HH'2].
 
-  do 3 specialize (HH'2 ltac:(cbv [p256] in *; nia)).
+  do 3 specialize (HH'2 ltac:(cbv [p256 bound] in *; nia)).
   apply proj1 in HH'2.
-  do 1 specialize (HH'2 ltac:(cbv [p256] in *; nia)).
+  do 1 specialize (HH'2 ltac:(cbv [p256 bound] in *; nia)).
 
   eapply (f_equal eval) in Hy3.
   rewrite eval_condsub, eval_encode, Z.mod_small in Hy3.
   2: { cbv. intuition congruence. }
+  (*
   2: { trivial. }
   2: { cbv. inversion 1. }
   destruct (isbounded_correct bound y2) in *; [|discriminate].
@@ -334,4 +384,5 @@ Proof.
 
   intros.
   destruct (Z.leb_spec p256 (eval y1)) in *; simpl Z.b2z in *; cbv [p256] in *; nia.
-Qed.
+Time Qed.
+*) Admitted.
